feat: add user-defined fallback procedure for the `grind` tactic
This PR introduces support for user-defined fallback code in the
`grind` tactic. The fallback code can be utilized to inspect the state
of failing `grind` subgoals and/or invoke user-defined
automation. Users can now write `grind on_failure <code>`, where
`<code>` should have the type `GoalM Unit`. See the modified tests in
this PR for examples.

tests/lean/run/grind_canon_types.lean
@@ -1,27 +1,22 @@
-import Lean
+import Lean.Meta.Tactic.Grind
 
 def g (s : Type) := s
 def f (a : α) := a
 
-open Lean Meta Elab Tactic Grind in
-elab "grind_test" : tactic => withMainContext do
-  let declName := (← Term.getDeclName?).getD `_main
-  Meta.Grind.preprocessAndProbe (← getMainGoal) declName do
-    let nodes ← filterENodes fun e => return e.self.isAppOf ``f
-    logInfo (nodes.toList.map (·.self))
-
+open Lean Meta Grind in
+def fallback : Fallback := do
+  let nodes ← filterENodes fun e => return e.self.isAppOf ``f
+  logInfo (nodes.toList.map (·.self))
+  (← get).mvarId.admit
 
 set_option pp.explicit true
 /--
 info: [@f Nat a, @f Nat b]
----
-warning: declaration uses 'sorry'
 -/
-#guard_msgs in
+#guard_msgs (info) in
 example (a b c d : Nat) : @f Nat a = b → @f (g Nat) a = c → @f (g Nat) b = d → a = b → False := by
   -- State should have only two `f`-applications: `@f Nat a`, `@f Nat b`
   -- Note that `@f (g Nat) b` has been canonicalized to `@f Nat b`.
   -- Thus, if `a` and `b` equivalence classes are merged, `grind` can still detect that
   -- `@f Nat a` and `@f Nat b` are equal too.
-  grind_test
-  sorry
+  grind on_failure fallback
